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1 Operators

We define ∆f(x) = f(x + 1)− f(x) as the first order finite difference. The symbol ∆ is
said to be the finite difference operator. Generally we define

∆rf(x) = ∆(∆r−1f(x)) (1)

as the r-order finite difference. Also we define the following operators:

1. Ef(x) = f(x + 1)

2. If(x) = f(x)

Hence

Enf(x) = f(x + n)

Inf(x) = f(x)

∆ = E − I

These operations will be very useful in proving some of the propositions below.

2 Finite Differences

Let’s start by finding a pattern in finite differences of various orders:

∆2f(x) = f(x + 2)− 2f(x + 1) + f(x)

∆3f(x) = f(x + 3)− 3f(x + 2) + 3f(x + 1)− f(x)

∆4f(x) = f(x + 4)− 4f(x + 3) + 6f(x + 2)− 4f(x + 1) + f(x)

As such, we propose the following:
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Proposition 1. Let r be a positive integer, then

∆nf(x) =
n∑

k=0

(−1)k
(
n

k

)
f(x + n− k) (2)

Proof. Since ∆ = E − I,

∆n = (E − I)n =
n∑

k=0

(−1)k
(
n

k

)
En−k �

Let’s look from a different perspective from Proposition 1, where we write a function
in terms of finite differences instead.

f(x + 1) = ∆f(x) + f(x)

f(x + 2) = ∆2f(x) + 2∆f(x) + f(x)

f(x + 3) = ∆3f(x) + 3∆2f(x) + 3∆f(x) + f(x)

Hence we propose the following:

Proposition 2. For any non-negative integer n,

f(x + n) =
n∑

k=0

(
n

k

)
∆kf(x) (3)

Proof. Since ∆ = E − I,

En = (∆ + I)n =
n∑

k=0

(
n

k

)
∆k �

Again, this directly brings us to

Proposition 3. For any non-negative integer n,

f(n) =
n∑

k=0

(
n

k

)
∆kf(0)

Proof. Proposition 2. x = 0. �
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We take one step further: Writing f(1) + · · ·+ f(n) as a sum of finite differences.

Proposition 4. The sum of the first n terms of f(n) is

f(1) + · · ·+ f(n) =
n∑

k=1

(
n

k

)
∆k−1f(1) (4)

Proof. Since ∆ = E − I,

E0 + · · ·+ En−1 =
En − I

E − I
=

(∆ + I)n − I

∆
=

n∑
k=0

(
n

k + 1

)
∆k �

3 Polynomials

Next let’s see what happens if we apply finite differences to polynomials:

f(x) = anx
n + . . .

∆f(x) = nanx
n−1 + . . .

∆2f(x) = n(n− 1)anx
n−2 + . . .

Proposition 5. If f(x) is an n-degree polynomial with leading coefficient an, then

∆nf(x) = n! · an (5)

Proof. Induct in terms of the leading coefficient.

The following proposition may be very useful and it is very straightforward. We can
use it to deal with the degree of a certain polynomial.

Proposition 6. If f(x) is an n-degree polynomial , then

∆n+1f(x) = 0 (6)

Proof. From proposition 5 we have ∆n+1f(x) = n! · an − n! · an = 0. �

From proposition 3, we can also generalise n to x, writing f(x) as a sum of what we
call finite difference polynomials (which is deep down just a binomial choose function!)
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Proposition 7. For any n-degree polynomial,

f(x) =
n∑

k=0

∆kf(0)

(
x

k

)
or simply

n∑
k=0

ck

(
x

k

)
Proof. f(x)−

∑n
k=0 ∆kf(0)

(
x
k

)
has n + 1 roots, hence 0. �

In fact, the expansion in proposition 7 is unique, and a polynomial is integer valued if
and only if ∀ci ∈ Z.

Example 1. Let m ≥ n be positive integers. Prove that

n∑
k=0

(−1)k
(
m− k

n

)(
n

k

)
= 1.

Solution. Note that ∆nf(x) is constant if we let

f(x) =

(
m− x

n

)
∴ LHS =

n∑
k=0

(−1)k
(
n

k

)
f(k)

= (−1)n∆nf(0)

= (−1)n∆nf(m− n)

=
n∑

k=0

(−1)k
(
n

k

)
f(m− n + k)

= 1 + 0 + 0 + 0 + · · · = 1 �

Example 2. Let P (x) be a polynomial of degree n such that

P (k) =

(
n + 1

k

)−1
for k = 0, 1, . . . , n. Find the value of P (n + 1).
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Solution. We start with

∆n+1P (x) = 0
n+1∑
i=0

(−1)i
(
n + 1

i

)
P (n + 1− i) = 0

P (n + 1) +
n+1∑
i=1

(−1)i = 0

∴ P (n + 1) =

{
0 if n is even;

1 if n is odd.

4 Falling Factorials

Let’s introduce and define falling factorials.

k(n) = k(k − 1) . . . (k − n + 1).

Yes, it is precisely another definition of P k
n . Take the finite difference

∆k(n) = (k + 1)(n) − k(n)

= (k + 1)k(n−1) − k(n−1)(k − n + 1)

= n · k(n−1)

and we see it resembles the definition of the derivative! Hence the backward process is
analogous, it is called finite integration.

Example 3. Find the value of

14 + · · ·+ n4.

Solution.

n∑
k=0

k4 =
n∑

k=0

(k(4) + 6k(3) + 7k(2) + k(1))

=
n∑

k=0

∆

(
1

5
k(5) +

3

2
k(4) +

7

3
k(3) +

1

2
k(2)
)

=

(
1

5
(n + 1)(5) +

3

2
(n + 1)(4) +

7

3
(n + 1)(3) +

1

2
(n + 1)(2)

)
− 0

=
1

30
n(n + 1)(2n + 1)(3n2 + 3n− 1)
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Example 4. Find the value of

23 + 53 + 83 + · · ·+ (3n + 2)3

Solution. We have f(n) = (3n + 2)3. Then

n∑
k=0

(3k + 2)3 =
n∑

k=1

(27k(3) + 135k(2) + 117k(1) + 8)

=
n∑

k=1

∆

(
27

4
k(4) + 45k(3) +

117

2
k(2) + 8k(1)

)
=

27

4
(n + 1)(4) + 45(n + 1)(3) +

117

2
(n + 1)(2) + 8(n + 1)(1)

=
1

4
(n + 1)(3n + 4)(9n2 + 21n + 8)

Example 5. Find the value of

n∑
k=0

(−1)k
(
n

k

)
kn+2

Solution. We basically want (I − E)nxn+2 = (−1)n∆nxn+2 evaluated at x = 0.

∆n(xn+2) = ∆n

(
x(n+2) +

{
n + 2
n + 1

}
x(n+1) +

{
n + 2
n

}
x(n) + · · ·

)
so the answer is

(−1)nn!

{
n + 2
n

}
= (−1)nn! · (n + 2)(n + 1)n(3n + 1)

24
= (−1)n · (n + 2)!(3n + 1)n

24
.
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